perennial/program_logic/staged_invariant_wp_nval.v
@@ -18,6 +18,7 @@ Context `{IRISG: !irisGS Λ Σ Ω, !generationGS Λ Σ}.
 Context `{!pri_invG IRISG}.
 Context `{!later_tokG IRISG}.
 Context `{!stagedG Σ}.
+Context `{!endisNG Σ Ω}.
 
 Lemma staged_inv_wp_nval E P Qs Qs' R :
   staged_value ⊤ Qs P -∗
@@ -31,7 +32,7 @@ Proof.
   iDestruct "Hinv" as (mj_wp_init mj_ishare Hlt) "#Hinv".
   rewrite /staged_inv.
   iDestruct (pri_inv_tok_disj_inv_half with "[$]") as %Hdisj.
-  iMod (pri_inv_acc with "[$]") as "(Hinner&Hclo)".
+  iMod (pri_cg_inv_acc with "[$]") as "(Hinner&Hclo)".
   { set_solver. }
   iEval (rewrite staged_inv_inner_unfold) in "Hinner".
   iDestruct "Hinner" as (?????) "(>Hown'&#Hsaved1'&#Hsaved2'&>Hstatus'&>Hitok_ishare&Hinner)".
