src/nextgen/nextgen_inv_promises.v
@@ -1,0 +1,110 @@
+From iris.algebra Require Import csum excl.
+From Perennial.base_logic.lib Require Import fancy_updates.
+From iris.proofmode Require Import tactics.
+From iris.bi Require Import fractional.
+From self.nextgen Require Import nextgen_promises.
+
+Definition endisR := agreeR (sumO unit unit).
+Class endisG Σ :=
+  EnDisG { endisG_inG : inG Σ (endisR); }.
+#[export] Existing Instance endisG_inG.
+Definition endisΣ : gFunctors := #[ GFunctor (endisR) ].
+Global Instance subG_endisΣ Σ : subG (endisΣ) Σ → endisG Σ.
+Proof. solve_inG. Qed.
+Class endisNG Σ Ω :=
+  EnDisNG { ng_endisG :> endisG Σ;
+            ng_deps :> genInDepsG Σ Ω (endisR) [#] }.
+Section endis.
+  Context `{os: !endisNG Σ Ω}.
+
+  (* the picked transformation makes enabled into disabled, and leaves disabled the same *)
+  Definition endis_trans_rel (t : endisR -> endisR) : Prop :=
+    ∀ a, t (to_agree a) ≡ to_agree (inr ()).
+  Definition endis_trans : endisR → endisR :=
+    λ a, agree_map (λ t, inr ()) a.
+
+  Global Instance endis_trans_cmramorphism : CmraMorphism endis_trans.
+  Proof.
+    apply agree_map_morphism.
+    intros ????. auto.
+  Qed.
+
+  Definition endis_en_def γ : iProp Σ := gen_own γ (to_agree (inl ())) ∗ rely_self γ endis_trans_rel.
+  Definition endis_en_aux : seal (@endis_en_def). Proof. by eexists. Qed.
+  Definition endis_en := endis_en_aux.(unseal).
+  Definition endis_en_eq : @endis_en = @endis_en_def := endis_en_aux.(seal_eq).
+
+  Definition endis_dis_def γ : iProp Σ := gen_own γ (to_agree (inr ())) ∗ rely_self γ endis_trans_rel.
+  Definition endis_dis_aux : seal (@endis_dis_def). Proof. by eexists. Qed.
+  Definition endis_dis := endis_dis_aux.(unseal).
+  Definition endis_dis_eq : @endis_dis = @endis_dis_def := endis_dis_aux.(seal_eq).
+
+  Lemma endis_en_alloc :
+    ⊢ |==> ∃ γ, endis_en γ.
+  Proof.
+    rewrite endis_en_eq.
+    iMod (own_gen_alloc (DS := [#]) (to_agree (inl ())) [#] [##] with "[]") as (γ) "[Hown Htok]".
+    { done. }
+    { iIntros (Hcontr). inversion Hcontr. }
+    iMod (token_strengthen_promise_0_deps _ _ endis_trans_rel with "Htok") as "Htok";auto.
+    { intros;done. }
+    { exists endis_trans. split;[apply _|]. intros ??.
+      rewrite /endis_trans agree_map_to_agree//. }
+    iModIntro. iExists γ. iFrame.
+    iApply rely_to_rely_self.
+    iApply token_to_rely. iFrame.
+  Qed.
+
+  Global Instance endis_dis_persistent γ : Persistent (endis_dis γ).
+  Proof. rewrite endis_dis_eq. apply _. Qed.
+  Global Instance endis_en_persistent γ : Persistent (endis_en γ).
+  Proof. rewrite endis_en_eq. apply _. Qed.
+
+  Lemma endis_en_shot_False γ :
+    endis_en γ -∗ endis_dis γ -∗ False.
+  Proof.
+    iIntros "H1 H2". rewrite endis_en_eq endis_dis_eq.
+    iDestruct "H1" as "[H1 _]".
+    iDestruct "H2" as "[H2 _]".
+    iDestruct (gen_own_valid_2 with "H1 H2") as %Hv%to_agree_op_valid.
+    inversion Hv.
+  Qed.
+
+  Global Instance endis_dis_timeless γ : Timeless (endis_dis γ).
+  Proof. rewrite endis_dis_eq. apply _. Qed.
+  Global Instance endis_en_timeless γ : Timeless (endis_en γ).
+  Proof. rewrite endis_en_eq. apply _. Qed.
+
+  Lemma nextgen_endis_en γ :
+    endis_en γ ⊢ ⚡==> endis_dis γ.
+  Proof.
+    rewrite endis_en_eq endis_dis_eq.
+    iIntros "[Hen Hrely]".
+    iModIntro.
+    iDestruct "Hen" as (t) "[Hpicked Hen]".
+    iDestruct "Hrely" as "[Hrely (%t' & %Ht & Hpicked')]".
+    iFrame.
+    iDestruct (gen_picked_in_agree with "Hpicked Hpicked'") as %->.
+    rewrite Ht. auto.
+  Qed.
+
+  Lemma nextgen_endis_dis γ :
+    endis_dis γ ⊢ ⚡==> endis_dis γ.
+  Proof.
+    rewrite endis_dis_eq.
+    iIntros "[Hen Hrely]".
+    iModIntro.
+    iDestruct "Hen" as (t) "[Hpicked Hen]".
+    iDestruct "Hrely" as "[Hrely (%t' & %Ht & Hpicked')]".
+    iFrame.
+    iDestruct (gen_picked_in_agree with "Hpicked Hpicked'") as %->.
+    rewrite Ht. auto.
+  Qed.
+
+  #[global]
+    Instance into_nextgen_endis_en γ : IntoNextgen _ _ := nextgen_endis_en γ.
+
+  #[global]
+    Instance into_nextgen_endis_dis γ : IntoNextgen _ _ := nextgen_endis_dis γ.
+    
+End endis.
